AccExc.v
@@ -1,0 +1,27 @@
+From Elo Require Import Core.
+
+From Elo Require Import AccessCore.
+From Elo Require Import AccessExclusivity.
+
+(* preservation -------------------------------------------------------------*)
+
+Local Lemma accexc_preservation_none : forall m ths tid t,
+  acc_exclusivity m ths ->
+  ths[tid] --[e_none]--> t ->
+  acc_exclusivity m ths[tid <- t].
+Proof.
+  intros ** ad tid1 tid2 T Had Hacc1 Hacc2.
+  repeat omicron; try solve invc_acc; eauto.
+  - admit.
+  - admit.
+  - admit.
+Qed.
+
+Theorem accexc_preservation : forall m1 m2 ths1 ths2 tid e,
+  acc_exclusivity m1 ths1 ->
+  m1 / ths1 ~~[tid, e]~~> m2 / ths2 ->
+  acc_exclusivity m2 ths2.
+Proof.
+  intros. invc_cstep; try invc_mstep.
+  -
+Qed.
