AccessExclusivity.v
@@ -1,0 +1,76 @@
+From Elo Require Import Core.
+
+From Elo Require Import Properties1.
+From Elo Require Import Properties2.
+
+From Elo Require Import AccessCore.
+
+(* ------------------------------------------------------------------------- *)
+(* exclusivity promises                                                      *)
+(* ------------------------------------------------------------------------- *)
+
+Definition acc_exclusivity (m : mem) (ths : threads) := forall ad tid1 tid2 T,
+  m[ad].T = `w&T` ->
+  access ad m ths[tid1] ->
+  access ad m ths[tid2] ->
+  tid1 = tid2.
+
+(* Two different threads cannot have xaccess to an address over the same adx. *)
+Definition xacc_exclusivity1 (m : mem) (ths : threads) :=
+  forall adx ad tid1 tid2 T,
+    m[ad].T = `w&T` ->
+    tid1 <> tid2 ->
+    xaccess adx ad m ths[tid1] ->
+    xaccess adx ad m ths[tid2] ->
+    False.
+
+(* 
+  A thread cannot have xaccess to an address with two distinct adxs.
+  Same goes for two distinct threads.
+*)
+Definition xacc_exclusivity2 (m : mem) (ths : threads) :=
+  forall adx1 adx2 ad tid1 tid2 T,
+    m[ad].T = `w&T` ->
+    adx1 <> adx2 ->
+    xaccess adx1 ad m ths[tid1] ->
+    xaccess adx2 ad m ths[tid2] ->
+    False.
+
+(* 
+  A thread cannot have xaccess to an address while a thread has access.
+*)
+Definition xacc_acc_exclusivity (m : mem) (ths : threads) :=
+  forall adx ad tid1 tid2 T,
+    m[ad].T = `w&T` ->
+    xaccess adx ad m ths[tid2] ->
+    access ad m ths[tid1] ->
+    False.
+
+(* ------------------------------------------------------------------------- *)
+(* xacc-exclusivity1 preservation                                            *)
+(* ------------------------------------------------------------------------- *)
+
+Theorem xaccexc1_preservation : forall m1 m2 ths1 ths2 tid e,
+  forall_threads ths2 (valid_addresses m2) ->
+  unique_initializers m2 ths2 ->
+  unique_critical_regions m2 ths2 ->
+  init_cr_exclusivity ths2 ->
+  (* --- *)
+  xacc_exclusivity1 m1 ths1 ->
+  m1 / ths1 ~~[tid, e]~~> m2 / ths2 ->
+  xacc_exclusivity1 m2 ths2.
+Proof.
+  intros * ? Hui Hucr Hice.
+  intros ** adx ad tid1 tid2 T Hptyp Hneq Hxacc1 Hxacc2.
+  destruct (Hice adx tid1 tid2) as [? ?].
+  assert (Hadx : adx < #m2) by eauto using xacc_adx_bounds.
+  assert ((one_init adx ths2[tid1]) \x/ (one_cr adx ths2[tid1]))
+    as [[? | ?] ?] by eauto using oneinit_xor_onecr_from_xacc;
+  assert ((one_init adx ths2[tid2]) \x/ (one_cr adx ths2[tid2]))
+    as [[? | ?] ?] by eauto using oneinit_xor_onecr_from_xacc.
+  - eauto using ui_oneinit_contradiction.
+  - eauto using nocr_onecr_contradiction.
+  - eauto using noinit_oneinit_contradiction.
+  - eauto using ucr_onecr_contradiction.
+Qed.
+
