AccessInheritance.v
@@ -1,0 +1,243 @@
+From Elo Require Import Core.
+
+From Elo Require Import Properties1.
+From Elo Require Import Properties2.
+
+From Elo Require Import AccessCore.
+
+Corollary noref_from_insert : forall m ths tid t ad te,
+  forall_threads ths (consistent_inits m) ->
+  no_uninitialized_references m ths ->
+  (* --- *)
+  ths[tid] --[e_insert ad te]--> t ->
+  forall_program m ths (no_ref ad).
+Proof.
+  eauto using insert_then_uninitialized.
+Qed.
+
+(* ------------------------------------------------------------------------- *)
+(* access inheritance                                                        *)
+(* ------------------------------------------------------------------------- *)
+
+Lemma acc_inheritance_subst : forall x Tx t tx ad,
+  access ad <{[x := tx] t}> ->
+  access ad <{call <{fn x Tx t}> tx}>.
+Proof.
+  intros. induction t; simpl in *;
+  try destruct str_eq_dec; try invc_acc; eauto using access;
+  aspecialize; repeat invc_acc; eauto using access.
+Qed.
+
+Lemma acc_inheritance_mem_add : forall m t ad T,
+  access ad (m +++ (None, T, false)) t ->
+  access ad m t.
+Proof.
+  intros * Hacc.
+  induction Hacc; eauto using access;
+  omicron; upsilon; eauto using access.
+Qed.
+
+Lemma acc_inheritance_mem_set1 : forall ad ad' m t t',
+  forall_memory m (no_ref ad') ->
+  no_ref ad' t ->
+  (* --- *)
+  access ad m[ad'.t <- t'] t ->
+  access ad m t.
+Proof.
+  intros * ? ? Hacc. induction Hacc; invc_noref; upsilon; eauto using access.
+Qed.
+
+Lemma acc_inheritance_mem_set2 : forall ad ad' m t t',
+  ~ access ad m t' ->
+  (* --- *)
+  access ad m[ad'.t <- t'] t ->
+  access ad m t.
+Proof.
+  intros * ? Hacc. induction Hacc; eauto using access;
+  repeat omicron; upsilon; eauto using access.
+Qed.
+
+Lemma acc_inheritance_mem_set3 : forall ad ad' m t t',
+  ~ access ad' m t ->
+  (* --- *)
+  access ad m[ad'.t <- t'] t ->
+  access ad m t.
+Proof.
+  intros * ? Hacc. induction Hacc; invc_nacc; sigma; eauto using access.
+Qed.
+
+Lemma acc_inheritance_mem_acq : forall ad ad' m t,
+  access ad m[ad'.X <- true] t ->
+  access ad m t.
+Proof.
+  intros * Hacc. induction Hacc; eauto using access;
+  (eapply acc_memR || eapply acc_memW); upsilon; eauto.
+Qed.
+
+Lemma acc_inheritance_mem_rel : forall ad ad' m t,
+  access ad m[ad'.X <- false] t ->
+  access ad m t.
+Proof.
+  intros * Hacc. induction Hacc; eauto using access;
+  (eapply acc_memR || eapply acc_memW); upsilon; eauto.
+Qed.
+
+(* ------------------------------------------------------------------------- *)
+
+Lemma acc_inheritance_none : forall ad m t1 t2,
+  access ad m t2 ->
+  t1 --[e_none]--> t2 ->
+  access ad m t1.
+Proof.
+  intros. ind_tstep; try invc_acc; eauto using acc_inheritance_subst, access.
+Qed.
+
+Lemma acc_inheritance_alloc : forall ad m t1 t2 T,
+  access ad (m +++ (None, T, false)) t2 ->
+  t1 --[e_alloc (#m) T]--> t2 ->
+  access ad m t1.
+Proof.
+  intros. ind_tstep; invc_acc; eauto using acc_inheritance_mem_add, access.
+Qed.
+
+Lemma acc_inheritance_insert : forall ad ad' m t t1 t2,
+  forall_memory m (no_ref ad') ->
+  no_ref ad' t1 ->
+  (* --- *)
+  ad <> ad' ->
+  access ad m[ad'.t <- t] t2 ->
+  t1 --[e_insert ad' t]--> t2 ->
+  access ad m t1.
+Proof.
+  intros. ind_tstep; invc_noref; invc_acc; eauto using access; upsilon;
+  eauto using acc_inheritance_mem_set1, access.
+Qed.
+
+Lemma acc_inheritance_read : forall ad ad' m t t1 t2,
+  well_typed_term t1 ->
+  (* --- *)
+  m[ad'].t = Some t ->
+  access ad m t2 ->
+  t1 --[e_read ad' t]--> t2 ->
+  access ad m t1.
+Proof.
+  intros * [T ?] **. gendep T.
+  ind_tstep; intros; repeat invc_typeof; try invc_acc; eauto using access;
+  destruct (nat_eq_dec ad' ad); subst; eauto using access.
+Qed.
+
+Lemma acc_inheritance_write : forall ad ad' m t t1 t2,
+  access ad m[ad'.t <- t] t2 ->
+  t1 --[e_write ad' t]--> t2 ->
+  access ad m t1.
+Proof.
+  intros. ind_tstep; invc_acc; eauto using access; upsilon.
+  - destruct (acc_dec ad' m t2); eauto using acc_inheritance_mem_set3, access.
+    destruct (acc_dec ad m t); eauto using acc_inheritance_mem_set2, access.
+    destruct (acc_dec ad m t1), (acc_dec ad m t2); eauto using access.
+    assert (~ access ad m <{call t1 t2}>) by eauto using nacc_call.
+Abort.
+
+(* ------------------------------------------------------------------------- *)
+(* xaccess inheritance                                                       *)
+(* ------------------------------------------------------------------------- *)
+
+Lemma xacc_inheritance_subst : forall m x Tx t tx ad adx,
+  no_inits t ->
+  no_crs   t ->
+  (* --- *)
+  xaccess adx ad m <{[x := tx] t}> ->
+  xaccess adx ad m <{call <{fn x Tx t}> tx}>.
+Proof.
+  intros. induction t; simpl in *; try destruct str_eq_dec;
+  invc_noinits; invc_nocrs; try invc_xacc;
+  repeat aspecialize; repeat invc_xacc; eauto using xaccess.
+Qed.
+
+Lemma xacc_inheritance_mem_add : forall m t adx ad T,
+  xaccess adx ad (m +++ (None, T, false)) t ->
+  xaccess adx ad m t.
+Proof.
+  intros * Hxacc. induction Hxacc; eauto using acc_inheritance_mem_add, xaccess.
+Qed.
+
+Lemma xacc_inheritance_mem_set1 : forall adx ad ad' m t t',
+  forall_memory m (no_ref ad') ->
+  no_ref ad' t ->
+  (* --- *)
+  xaccess adx ad m[ad'.t <- t'] t ->
+  xaccess adx ad m t.
+Proof.
+  intros * ? ? Hxacc. induction Hxacc; invc_noref; eauto using xaccess;
+  eauto using acc_inheritance_mem_set1, xaccess.
+Qed.
+
+Lemma xacc_inheritance_mem_set2 : forall adx ad ad' m t t',
+  ~ access ad m t' ->
+  (* --- *)
+  xaccess adx ad m[ad'.t <- t'] t ->
+  xaccess adx ad m t.
+Proof.
+  intros * ? Hxacc. induction Hxacc;
+  eauto using acc_inheritance_mem_set2, xaccess.
+Qed.
+
+(* ------------------------------------------------------------------------- *)
+
+Lemma xacc_inheritance_none : forall adx ad m t1 t2,
+  valid_blocks t1 ->
+  (* --- *)
+  xaccess adx ad m t2 ->
+  t1 --[e_none]--> t2 ->
+  xaccess adx ad m t1.
+Proof.
+  intros. ind_tstep; repeat invc_vb; try invc_xacc;
+  eauto using acc_inheritance_none, xacc_inheritance_subst, xaccess.
+Qed.
+
+Lemma xacc_inheritance_alloc : forall adx ad m t1 t2 T,
+  adx <> #m ->
+  xaccess adx ad (m +++ (None, T, false)) t2 ->
+  t1 --[e_alloc (#m) T]--> t2 ->
+  xaccess adx ad m t1.
+Proof.
+  intros. ind_tstep; invc_xacc;
+  eauto using acc_inheritance_alloc, xacc_inheritance_mem_add, xaccess.
+Qed.
+
+Lemma xacc_inheritance_insert : forall adx ad ad' m t t1 t2,
+  forall_memory m (no_ref ad') ->
+  no_ref ad' t1 ->
+  (* --- *)
+  ad <> ad' ->
+  xaccess adx ad m[ad'.t <- t] t2 ->
+  t1 --[e_insert ad' t]--> t2 ->
+  xaccess adx ad m t1.
+Proof.
+  intros. ind_tstep; invc_noref; inv_xacc; eauto using xaccess;
+  eauto using acc_inheritance_insert, xacc_inheritance_mem_set1, xaccess.
+Qed.
+
+Lemma xacc_inheritance_read : forall adx ad ad' m t t1 t2,
+  forall_memory m value ->
+  forall_memory m valid_blocks ->
+  well_typed_term t1 ->
+  (* --- *)
+  m[ad'].t = Some t ->
+  xaccess adx ad m t2 ->
+  t1 --[e_read ad' t]--> t2 ->
+  xaccess adx ad m t1.
+Proof.
+  intros. ind_tstep; intros; invc_wtt; try invc_xacc;
+  eauto using acc_inheritance_read, xaccess.
+  exfalso. eauto using xacc_value_contradiction.
+Qed.
+
+Lemma xacc_inheritance_write : forall adx ad ad' m t t1 t2,
+  ad <> ad' ->
+  xaccess adx ad m[ad'.t <- t] t2 ->
+  t1 --[e_write ad' t]--> t2 ->
+  xaccess adx ad m t1.
+Proof.
+  intros. ind_tstep; invc_xacc; eauto using xaccess; upsilon.
+Abort.
