Promise.v
@@ -2,17 +2,48 @@ From Elo Require Import Core.
 
 From Elo Require Import Properties1.
 
-From Elo Require Import NoUninitRefs.
-From Elo Require Import ConsistentRefs.
-
+From Elo Require Import NoRef.
 From Elo Require Import NoWRef.
+From Elo Require Import NoUninitRefs.
+From Elo Require Import ConsistentInits.
+From Elo Require Import ConsistentRefs.
+From Elo Require Import InitCRExclusivity.
+
 From Elo Require Import AccessCore.
 From Elo Require Import PointerTypes.
 From Elo Require Import Inheritance.
+From Elo Require Import SafeNewX.
 
 (* ------------------------------------------------------------------------- *)
 (* exclusivity-promise                                                       *)
 (* ------------------------------------------------------------------------- *)
+
+(*
+xaccess adx ad m t ->
+one_cr adx t.
+
+no_cr adx t ->
+xaccess adx ad m t ->
+False.
+
+write ----------------------- read
+
+Definition exclusivity_promise0 (m : mem) (ths : threads) :=
+  forall adx ad tid1 tid2 T,
+    tid1 <> tid2 ->
+    m[ad].T = `w&T` ->
+    xaccess adx ad m ths[tid1] ->
+    xaccess adx ad m ths[tid2] ->
+    False.
+
+Definition exclusivity_promise0 (m : mem) (ths : threads) :=
+  forall adx ad tid1 tid2 T,
+    adx <> adx' ->
+    m[ad].T = `w&T` ->
+    xaccess adx  ad m ths[tid1] ->
+    xaccess adx' ad m ths[tid2] ->
+    False.
+*)
 
 Definition exclusivity_promise (m : mem) (ths : threads) :=
   forall adx ad tid1 tid2 T,
@@ -34,14 +65,7 @@ Proof.
   eauto using acc_inheritance_none, xacc_inheritance_none.
 Qed.
 
-Local Lemma noref_acc_contradiction : forall m t ad,
-  forall_memory m (no_ref ad) ->
-  no_ref ad t ->
-  access ad m t ->
-  False.
-Proof.
-  intros * ? ? H. induction H; invc_noref; eauto.
-Qed.
+(* ------------------------------------------------------------------------- *)
 
 Local Lemma noref_xacc_contradiction : forall m t adx ad,
   forall_memory m (no_ref ad) ->
@@ -51,13 +75,6 @@ Local Lemma noref_xacc_contradiction : forall m t adx ad,
 Proof.
   intros * ? ? H. induction H; invc_noref; eauto using noref_acc_contradiction.
 Qed.
-
-
-
-
-
-
-
 
 Lemma vad_nacc_length : forall m t,
   forall_memory m (valid_addresses m) ->
@@ -80,16 +97,7 @@ Proof.
   induction Hxacc; invc_vad; eauto using vad_nacc_length.
 Qed.
 
-Lemma xacc_noinit_nocr_contradiction : forall adx ad m t,
-  no_init adx t ->
-  no_cr   adx t ->
-  xaccess adx ad m t ->
-  False.
-Proof.
-  intros. induction t; invc_noinit; inv_nocr; invc_xacc; eauto.
-Qed.
-
-Lemma todo1 : forall ad m t T,
+Lemma acc_nowref_contradiction : forall ad m t T,
   forall_memory m value ->
   forall_memory m (consistent_references m) ->
   consistent_references m t ->
@@ -105,43 +113,42 @@ Proof.
   eauto using wacc_safe_contradiction.
 Qed.
 
-Lemma todo : forall ad m t T1 T2,
+Lemma alloc_xacc_contradiciton : forall adx ad m t1 t2 T Te,
   forall_memory m value ->
   forall_memory m (consistent_references m) ->
-  consistent_references m t ->
+  consistent_references m t1 ->
   (* --- *)
-  m[ad].T = `w&T1` ->
-  no_cr (#m) t ->
-  one_init (#m) t ->
-  no_wrefs t ->
-  xaccess (#m) ad (m +++ (None, T2, false)) t ->
+  m[ad].T = `w&T` ->
+  safe_newx t1 ->
+  t1 --[e_alloc adx Te]--> t2 ->
+  xaccess adx ad m t2 ->
+  one_init adx t2 ->
+  no_cr    adx t2 ->
   False.
 Proof.
-  intros * ? ? ? ? ? ? ? Hxacc. induction Hxacc;
-  try solve [
-    invc_cr; invc_nowrefs; invc_nocr; inv_oneinit;
-    eauto using xacc_noinit_nocr_contradiction
-  ].
-  invc_cr. invc_nowrefs. invc_nocr. invc_oneinit; eauto.
-  eapply todo1; eauto.
-
-Abort.
-
-
-
-
-
-
+  intros. ind_tstep; invc_cr; invc_snx; invc_xacc; invc_oneinit; invc_nocr;
+  eauto;
+  eauto using xacc_noinit_nocr_contradiction;
+  eauto using noinit_inheritance_alloc, noinit_to_oneinit,
+    noinit_oneinit_contradiction.
+  eauto using acc_nowref_contradiction.
+Qed.
 
 Local Lemma ep_preservation_alloc : forall m ths tid t T,
+  forall_memory m value ->
+  forall_memory m (consistent_references m) ->
   forall_threads ths (valid_addresses m) ->
+  forall_threads ths valid_blocks ->
+  forall_threads ths (consistent_references m) ->
+  forall_threads ths safe_newx ->
   no_uninitialized_references m ths ->
+  init_cr_exclusivity ths ->
   (* --- *)
   exclusivity_promise m ths ->
   ths[tid] --[e_alloc (#m) T]--> t ->
   exclusivity_promise (m +++ (None, T, false)) ths[tid <- t].
 Proof.
-  intros * Hvad Hnur Hep Htstep.
+  intros until 7. intros Hice. intros Hep Htstep.
   assert (Hvad' : valid_addresses (m +++ (None, T, false)) t)
     by eauto using vad_preservation_alloc.
   assert
@@ -158,14 +165,98 @@ Proof.
     + specialize (Hths tid1). sigma. eauto using noref_acc_contradiction.
   - repeat omicron; try solve [invc_acc || invc_xacc].
     + destruct (nat_eq_dec (#m) adx); subst.
-      * assert (no_init (#m) ths[tid2]) by eauto using vad_noinit_ad.
+      * assert (xaccess (#m) ad m t) by eauto using xacc_inheritance_mem_add.
+        assert (no_init (#m) ths[tid2]) by eauto using noinit_from_vad.
         assert (one_init (#m) t) by eauto using noinit_to_oneinit.
-        admit.
+        eapply ice_preservation_alloc in Hice; eauto.
+        specialize (Hice (#m) tid2 tid2) as [? ?]; sigma.
+        eauto using alloc_xacc_contradiciton.
       * eauto using acc_inheritance_alloc, xacc_inheritance_alloc.
     + eauto using acc_inheritance_alloc, xacc_inheritance_mem_add.
     + destruct (nat_eq_dec (#m) adx); subst.
-      * admit.
+      * assert (xaccess (#m) ad m t) by eauto using xacc_inheritance_mem_add.
+        assert (no_init (#m) ths[tid2]) by eauto using noinit_from_vad.
+        assert (one_init (#m) t) by eauto using noinit_to_oneinit.
+        eapply ice_preservation_alloc in Hice; eauto.
+        specialize (Hice (#m) tid2 tid2) as [? ?]; sigma.
+        eauto using alloc_xacc_contradiciton.
       * eauto using xacc_inheritance_alloc, acc_inheritance_mem_add.
     + eauto using acc_inheritance_mem_add, xacc_inheritance_mem_add.
+Qed.
+
+(* ------------------------------------------------------------------------- *)
+
+Local Lemma insert_acc_xacc_contradiction : forall adx ad m t t1 t2,
+  forall_memory m (no_ref ad) ->
+  no_ref ad t1 ->
+  t1 --[e_insert ad t]--> t2 ->
+  access ad m[ad.t <- t] t2 ->
+  xaccess adx ad m[ad.t <- t] t2 ->
+  False.
+Proof.
+  intros. ind_tstep; invc_noref; invc_acc; invc_xacc;
+  eauto using acc_inheritance_mem_set1, noref_acc_contradiction;
+  eauto using xacc_inheritance_mem_set1, noref_xacc_contradiction.
+Qed.
+
+Local Lemma ep_preservation_insert : forall m ths tid t ad te,
+  forall_threads ths (consistent_inits m) ->
+  no_uninitialized_references m ths ->
+  (* --- *)
+  exclusivity_promise m ths ->
+  ths[tid] --[e_insert ad te]--> t ->
+  exclusivity_promise m[ad.t <- te] ths[tid <- t].
+Proof.
+  intros until 2. rename ad into ad'.
+  intros Hep Htstep adx ad tid1 tid2 T Had Hxacc Hacc.
+  assert (forall_program m ths (no_ref ad')) as [? ?]
+    by eauto using noref_from_insert.
+  repeat omicron; upsilon; try solve [invc Had | invc_acc | invc_xacc].
+  - eauto using insert_acc_xacc_contradiction.
+  - eauto using acc_inheritance_insert, xacc_inheritance_insert.
+  - eauto using xacc_inheritance_mem_set1, noref_xacc_contradiction.
+  - eauto using acc_inheritance_insert, xacc_inheritance_mem_set1.
+  - eauto using acc_inheritance_mem_set1, noref_acc_contradiction.
+  - eauto using acc_inheritance_mem_set1, xacc_inheritance_insert.
+  - eauto using xacc_inheritance_mem_set1, noref_xacc_contradiction.
+  - eauto using acc_inheritance_mem_set1, xacc_inheritance_mem_set1.
+Qed.
+
+(* ------------------------------------------------------------------------- *)
+
+Local Lemma ep_preservation_read : forall m ths tid t ad te,
+  forall_memory m value ->
+  forall_memory m valid_blocks ->
+  forall_threads ths well_typed_term ->
+  (* --- *)
+  m[ad].t = Some te ->
+  exclusivity_promise m ths ->
+  ths[tid] --[e_read ad te]--> t ->
+  exclusivity_promise m ths[tid <- t].
+Proof.
+  intros until 4. rename ad into ad'.
+  intros Hep Htstep adx ad tid1 tid2 T Had Hxacc Hacc.
+  repeat omicron; try solve [invc_acc | invc_xacc];
+  eauto using acc_inheritance_read, xacc_inheritance_read.
+Qed.
+
+(* ------------------------------------------------------------------------- *)
+
+Local Lemma ep_preservation_write : forall m ths tid t ad te,
+  exclusivity_promise m ths ->
+  ths[tid] --[e_write ad te]--> t ->
+  exclusivity_promise m[ad.t <- te] ths[tid <- t].
+Proof.
+  intros *. rename ad into ad'.
+  intros Hep Htstep adx ad tid1 tid2 T Had Hxacc Hacc.
+  repeat omicron; upsilon; try solve [invc Had | invc_acc | invc_xacc].
+  - destruct (acc_dec ad m ths[tid2]), (xacc_dec adx ad m ths[tid2]); eauto.
+  - admit.
+  - admit.
+  - admit.
+  - admit.
+  - admit.
+  - admit.
+  - admit.
 Qed.
 
