Properties2.v
@@ -1,0 +1,10 @@
+From Elo Require Export NoRef.
+From Elo Require Export NoWRef.
+From Elo Require Export NoUninitRefs.
+From Elo Require Export UniqueInits.
+From Elo Require Export UniqueCRs.
+From Elo Require Export ConsistentInits.
+From Elo Require Export ConsistentRefs.
+From Elo Require Export Soundness.
+From Elo Require Export InitCR.
+
